consistently use \<gamma> for matchers

PF.thy
@@ -17,38 +17,38 @@ fun matches :: "('a, 'p) matcher \<Rightarrow> 'a match_expr \<Rightarrow> 'p \<
 "matches \<gamma> (Match e) p \<longleftrightarrow> \<gamma> e p" |
 "matches _ MatchAny _ \<longleftrightarrow> True"
 
-lemma "matches m (MatchOr e1 e2) p \<longleftrightarrow> matches m e1 p \<or> matches m e2 p" unfolding MatchOr_def by auto
+lemma "matches \<gamma> (MatchOr e1 e2) p \<longleftrightarrow> matches \<gamma> e1 p \<or> matches \<gamma> e2 p" unfolding MatchOr_def by auto
 
 fun filter_spec :: "'a ruleset \<Rightarrow> ('a, 'p) matcher \<Rightarrow> 'p \<Rightarrow> decision \<Rightarrow> decision" where
-"filter_spec [] m p d = d" |
-"filter_spec ((PfRule r)#ls) m p d = (if (matches m (pf_rule.get_match r) p)
+"filter_spec [] \<gamma> p d = d" |
+"filter_spec ((PfRule r)#ls) \<gamma> p d = (if (matches \<gamma> (pf_rule.get_match r) p)
                                        then (if (pf_rule.get_quick r)
                                               then (action_to_decision (pf_rule.get_action r) d)
-                                              else (filter_spec ls m p (action_to_decision (pf_rule.get_action r) d)))
-                                       else filter_spec ls m p d)" |
-"filter_spec ((Anchor r b)#ls) m p d = (if (matches m (anchor_rule.get_match r) p)
-                                         then (filter_spec (b@ls) m p d)
-                                         else filter_spec ls m p d)"
+                                              else (filter_spec ls \<gamma> p (action_to_decision (pf_rule.get_action r) d)))
+                                       else filter_spec ls \<gamma> p d)" |
+"filter_spec ((Anchor r b)#ls) \<gamma> p d = (if (matches \<gamma> (anchor_rule.get_match r) p)
+                                         then (filter_spec (b@ls) \<gamma> p d)
+                                         else filter_spec ls \<gamma> p d)"
 
 fun filter :: "'a ruleset \<Rightarrow> ('a, 'p) matcher \<Rightarrow> 'p \<Rightarrow> decision_wrap \<Rightarrow> decision_wrap" where
 "filter _ _ _ (Final d) = Final d" |
 "filter [] _ _ d = d" |
-"filter (l#ls) m p (Preliminary d) =
-  filter ls m p (case l of
-                  (PfRule r) \<Rightarrow> (if (matches m (pf_rule.get_match r) p)
+"filter (l#ls) \<gamma> p (Preliminary d) =
+  filter ls \<gamma> p (case l of
+                  (PfRule r) \<Rightarrow> (if (matches \<gamma> (pf_rule.get_match r) p)
                                                then (if (get_quick r)
                                                       then (Final (action_to_decision (get_action r) d))
                                                       else (Preliminary (action_to_decision (get_action r) d)))
                                                else (Preliminary d))
-                  | (Anchor r body) \<Rightarrow> (if (matches m (anchor_rule.get_match r) p)
-                                                    then filter (body) m p (Preliminary d)
+                  | (Anchor r body) \<Rightarrow> (if (matches \<gamma> (anchor_rule.get_match r) p)
+                                                    then filter (body) \<gamma> p (Preliminary d)
                                                     else (Preliminary d)))"
 
 case_of_simps filter_cases: filter.simps
 
 
 lemma filter_chain:
-  shows "filter (l1@l2) m p d = filter l2 m p (filter l1 m p d)"
+  shows "filter (l1@l2) \<gamma> p d = filter l2 \<gamma> p (filter l1 \<gamma> p d)"
 proof(induction l1 arbitrary: d)
   case Nil
   then show ?case
@@ -71,7 +71,7 @@ next
     proof(cases a)
 case (PfRule r)
   then show ?thesis
-    proof(cases "matches m (pf_rule.get_match r) p")
+    proof(cases "matches \<gamma> (pf_rule.get_match r) p")
     case True
     then show ?thesis unfolding PfRule using Prem IH by auto
   next
@@ -81,7 +81,7 @@ case (PfRule r)
 next
   case (Anchor r l)
   then show ?thesis
-  proof(cases "matches m (anchor_rule.get_match r) p")
+  proof(cases "matches \<gamma> (anchor_rule.get_match r) p")
     case True
     then show ?thesis using Prem IH by auto
   next
@@ -92,17 +92,17 @@ qed
 qed
 qed
 
-lemma "filter_spec rules m p start_decision = unwrap_decision (filter rules m p (Preliminary start_decision))"
-proof(induction rules m p start_decision rule: filter_spec.induct)
-  case (1 m p d)
+lemma "filter_spec rules \<gamma> p start_decision = unwrap_decision (filter rules \<gamma> p (Preliminary start_decision))"
+proof(induction rules \<gamma> p start_decision rule: filter_spec.induct)
+  case (1 \<gamma> p d)
   then show ?case by simp
 next
-  case (2 ls m p d)
+  case (2 ls \<gamma> p d)
   then show ?case by simp
 next
-  case IH: (3 r b ls m p d)
+  case IH: (3 r b ls \<gamma> p d)
   then show ?case
-  proof(cases "matches m (anchor_rule.get_match r) p")
+  proof(cases "matches \<gamma> (anchor_rule.get_match r) p")
     case True
     then show ?thesis using IH by (auto simp: filter_chain)
   next
@@ -113,23 +113,23 @@ qed
 
 (* default behavior is Accept *)
 definition pf :: "'a ruleset \<Rightarrow> ('a, 'p) matcher \<Rightarrow> 'p \<Rightarrow> decision" where
-"pf rules m packet = unwrap_decision (filter rules m packet (Preliminary Accept))"
+"pf rules \<gamma> packet = unwrap_decision (filter rules \<gamma> packet (Preliminary Accept))"
 
 definition filter' :: "'a ruleset \<Rightarrow> ('a \<Rightarrow> bool) \<Rightarrow> decision_wrap \<Rightarrow> decision_wrap" where
-"filter' rules m d = filter rules (\<lambda>a p. m a) () d"
+"filter' rules \<gamma> d = filter rules (\<lambda>a p. \<gamma> a) () d"
 
-lemma matches_equiv[simp]: "matches (\<lambda>a p. m a packet) me () = matches m me packet"
+lemma matches_equiv[simp]: "matches (\<lambda>a p. \<gamma> a packet) me () = matches \<gamma> me packet"
   by (induction me, auto)
 
-lemma filter_filter'_eq[simp]: "filter' rules (\<lambda>a. m a packet) d = filter rules m packet d"
+lemma filter_filter'_eq[simp]: "filter' rules (\<lambda>a. \<gamma> a packet) d = filter rules \<gamma> packet d"
 unfolding filter'_def
-by (induction rules m packet d rule: filter.induct) (auto split: line.splits)
+by (induction rules \<gamma> packet d rule: filter.induct) (auto split: line.splits)
 
 (* default behavior is Accept *)
 definition pf' :: "'a ruleset \<Rightarrow> ('a \<Rightarrow> bool) \<Rightarrow> decision" where
-"pf' rules m = unwrap_decision (filter' rules m (Preliminary Accept))"
+"pf' rules \<gamma> = unwrap_decision (filter' rules \<gamma> (Preliminary Accept))"
 
-lemma "pf rules m packet = pf' rules (\<lambda>a. m a packet)"
+lemma "pf rules \<gamma> packet = pf' rules (\<lambda>a. \<gamma> a packet)"
   unfolding pf_def pf'_def
   by simp
 
