Util.thy
@@ -6,7 +6,7 @@ begin
 definition ruleset_equiv :: "'a ruleset \<Rightarrow> 'a ruleset \<Rightarrow> bool" ("_ \<simeq> _") where
 "(l1 \<simeq> l2) \<longleftrightarrow> (pf' l1 = pf' l2)"
 
-lemma ruleset_equivI[intro]: "(\<And>m. pf' l1 m = pf' l2 m) \<Longrightarrow> l1 \<simeq> l2"
+lemma ruleset_equivI[intro]: "(\<And>m. pf' l1 \<gamma> = pf' l2 \<gamma>) \<Longrightarrow> l1 \<simeq> l2"
   unfolding ruleset_equiv_def by auto
 
 lemma ruleset_equiv_refl[intro, simp]: "l \<simeq> l" by auto
